Revamped  Message Dependencies

theories/VLSM/Core/MessageDependencies.v
@@ -1,7 +1,7 @@
 From stdpp Require Import prelude.
-From Coq Require Import FinFun.
-From VLSM Require Import Lib.Preamble Lib.StdppListSet Lib.Measurable.
-From VLSM Require Import Core.VLSM Core.Composition Core.Equivocation.
+From Coq Require Import FinFun Relations.Relation_Operators.
+From VLSM.Lib Require Import Preamble ListExtras FinFunExtras StdppListSet Measurable.
+From VLSM.Core Require Import VLSM VLSMProjections Composition ProjectionTraces SubProjectionTraces Equivocation.
 
 (** * VLSM Message Dependencies
 
@@ -10,14 +10,18 @@ Assumes that each message has an associated set of [message_dependencies].
 
 *)
 
-Section message_dependencies.
+Section sec_message_dependencies.
 
 Context
   {message : Type}
   (message_dependencies : message -> set message)
   (X : VLSM message)
-  {Hbo : HasBeenObservedCapability X}
+  {Hbs : HasBeenSentCapability X}
+  {Hbr : HasBeenReceivedCapability X}
+  (Hbo : HasBeenObservedCapability X := HasBeenObservedCapability_from_sent_received X)
   .
+
+Existing Instance Hbo.
 
 (**
 [MessageDependencies] characterize a <<message_dependencies>> function
@@ -51,9 +55,8 @@ observed all of <<m>>'s dependencies.
 Definition message_dependencies_full_node_condition
   (s : vstate X)
   (m : message)
-  : Prop
-  := forall dm, dm ∈ message_dependencies m ->
-    has_been_observed X s dm.
+  : Prop :=
+  forall dm, dm ∈ message_dependencies m -> has_been_observed X s dm.
 
 (** A VLSM has the [message_dependencies_full_node_condition_prop]
 if the validity of receiving a message in a state implies the
@@ -63,4 +66,444 @@ Definition message_dependencies_full_node_condition_prop : Prop :=
   forall l s m,
   vvalid X l (s, Some m) -> message_dependencies_full_node_condition s m.
 
-End message_dependencies.
+(** Membership to the message_dependencies of a message induces a dependency
+relation.
+*)
+Definition msg_dep_rel : relation message :=
+  fun m1 m2 => m1 ∈ message_dependencies m2.
+
+(** The transitive closure of the [msg_dep_rel]ation is a happens-before
+relation.
+*)
+Definition msg_dep_happens_before : relation message := flip (clos_trans _ (flip msg_dep_rel)).
+
+(** Unrolling one the [msg_dep_happens_before] relation one step. *)
+Lemma msg_dep_happens_before_iff_one x z
+  : msg_dep_happens_before x z <->
+    msg_dep_rel x z \/ exists y, msg_dep_happens_before x y /\ msg_dep_rel y z.
+Proof.
+  split.
+  - intros Hhb.
+    apply Operators_Properties.clos_trans_t1n in Hhb.
+    inversion Hhb; subst.
+    + left. assumption.
+    + right.
+      exists y.
+      split; [|assumption].
+      apply Operators_Properties.clos_t1n_trans.
+      assumption.
+  - intros Hhb.
+    apply Operators_Properties.clos_t1n_trans.
+    destruct Hhb as [Hone | [y [Hhb Hone]]].
+    + apply t1n_step. assumption.
+    + apply t1n_trans with y; [assumption|].
+      apply Operators_Properties.clos_trans_t1n.
+      assumption.
+Qed.
+
+Global Instance msg_dep_happens_before_transitive : Transitive msg_dep_happens_before.
+Proof.
+  apply flip_Transitive.
+  intros m1 m2 m3.
+  apply t_trans.
+Qed.
+
+(** If the [msg_dep_rel]ation reflects a predicate <<P>> and the induced
+[msg_dep_happens_before] is [well_founded], then if <<P>> holds for a message,
+it will hold for all its dependencies. *)
+Lemma msg_dep_happens_before_reflect
+  (P : message -> Prop)
+  (Hreflects : forall dm m, msg_dep_rel dm m -> P m -> P dm)
+  : forall dm m, msg_dep_happens_before dm m -> P m -> P dm.
+Proof.
+  intros dm m Hdm.
+  apply Operators_Properties.clos_trans_t1n in Hdm.
+  induction Hdm; [apply Hreflects; assumption|].
+  intro Hpx.
+  apply IHHdm.
+  revert Hpx.
+  apply Hreflects.
+  assumption.
+Qed.
+
+(** In the absence of initial messages, and if [msg_dep_rel] reflects the
+pre-loaded message property, then it also reflects the [valid_message_prop]erty.
+*)
+Lemma msg_dep_reflects_validity
+  (HMsgDep : MessageDependencies)
+  (no_initial_messages_in_X : forall m, ~ vinitial_message_prop X m)
+  (P : message -> Prop)
+  (Hreflects : forall dm m, msg_dep_rel dm m -> P m -> P dm)
+  (Hbr_pre := preloaded_HasBeenReceivedCapability Hbr)
+  (Hbs_pre := preloaded_HasBeenSentCapability Hbs)
+  (Hbo_pre := HasBeenObservedCapability_from_sent_received (pre_loaded_vlsm X P))
+  : forall dm m, msg_dep_rel dm m ->
+    valid_message_prop (pre_loaded_vlsm X P) m ->
+    valid_message_prop (pre_loaded_vlsm X P) dm.
+Proof.
+  intros dm m Hdm.
+  rewrite emitted_messages_are_valid_iff.
+  rewrite can_emit_iff.
+  intros [Hinit | [s Hproduce]].
+  - rewrite emitted_messages_are_valid_iff.
+    left.
+    right.
+    apply Hreflects with m; [assumption|].
+    destruct Hinit as [Hinit | Hp]; [|assumption].
+    elim (no_initial_messages_in_X m).
+    assumption.
+  - apply (observed_valid (pre_loaded_vlsm X P)) with (s := s)
+    ; [exists (Some m); apply can_produce_valid; eassumption|].
+    cut (has_been_observed X s dm).
+    {
+      intros [Hsent | Hreceived]; [left|right].
+      - clear -Hsent. destruct Hbs. assumption.
+      - clear -Hreceived. destruct Hbr. assumption.
+    }
+    apply message_dependencies_are_necessary with m; [|assumption].
+    revert Hproduce.
+    apply VLSM_incl_can_produce.
+    apply pre_loaded_vlsm_incl_pre_loaded_with_all_messages.
+Qed.
+
+(** Under [MessageDependencies] assumptions, if a message [has_been_sent]
+in a state <<s>>, then any of its direct dependencies [has_been_observed].
+*)
+Lemma msg_dep_has_been_sent
+  (HMsgDep : MessageDependencies)
+  s
+  (Hs : valid_state_prop (pre_loaded_with_all_messages_vlsm X) s)
+  m
+  (Hsent : has_been_sent X s m)
+  : forall dm, msg_dep_rel dm m -> has_been_observed X s dm.
+Proof.
+  intros dm Hdm.
+  cut (exists item, can_produce (pre_loaded_with_all_messages_vlsm X) (destination item) m /\ in_futures (pre_loaded_with_all_messages_vlsm X) (destination item) s).
+  {
+    intros [s_dm [Hproduce Hfutures]].
+    eapply in_futures_preserving_oracle_from_stepwise; [|eassumption|].
+    - apply has_been_observed_from_sent_received_stepwise_props.
+    - apply message_dependencies_are_necessary with m; assumption.
+  }
+  apply proper_sent in Hsent; [|assumption].
+  apply valid_state_has_trace in Hs as [is [tr Htr]].
+  specialize (Hsent _ _ Htr).
+  apply Exists_exists in Hsent as [item [Hitem Houtput]].
+  exists item.
+  split; cycle 1.
+  - eapply elem_of_trace_in_futures_left; [|eassumption].
+    apply Htr.
+  - unfold can_produce.
+    replace (Some m) with (output item) by assumption.
+    eapply can_produce_from_valid_trace; [|eassumption].
+    eapply valid_trace_forget_last.
+    apply Htr.
+Qed.
+
+(** If the [valid]ity predicate has the [message_dependencies_full_node_condition_prop]erty,
+then if a message [has_been_received] in a state <<s>>, any of its direct
+dependencies [has_been_observed].
+*)
+Lemma full_node_has_been_received
+  (Hfull : message_dependencies_full_node_condition_prop)
+  s
+  (Hs : valid_state_prop (pre_loaded_with_all_messages_vlsm X) s)
+  m
+  (Hreceived : has_been_received X s m)
+  : forall dm, msg_dep_rel dm m -> has_been_observed X s dm.
+Proof.
+  intros dm Hdm.
+  apply proper_received in Hreceived; [|assumption].
+  apply valid_state_has_trace in Hs as [is [tr Htr]].
+  specialize (Hreceived _ _ Htr).
+  apply Exists_exists in Hreceived as [item [Hitem Hinput]].
+  apply elem_of_list_split in Hitem as [pre [suf Heqtr]].
+  eapply in_futures_preserving_oracle_from_stepwise with (s1 := finite_trace_last is pre)
+  ; [apply has_been_observed_from_sent_received_stepwise_props|..].
+  - exists (item  :: suf).
+    eapply finite_valid_trace_from_to_app_split.
+    rewrite <- Heqtr.
+    apply Htr.
+  - eapply Hfull; [|eassumption].
+    replace (Some m) with (input item) by assumption.
+    clear Hinput.
+    eapply (input_valid_transition_is_valid (pre_loaded_with_all_messages_vlsm X)).
+    eapply input_valid_transition_to; [|simpl; eassumption].
+    eapply valid_trace_forget_last.
+    apply Htr.
+Qed.
+
+(** By combining Lemmas [msg_dep_has_been_sent] and [full_node_has_been_received],
+[msg_dep_rel] reflects the [has_been_observed] predicate.
+*)
+Lemma msg_dep_full_node_reflects_has_been_observed
+  (HMsgDep : MessageDependencies)
+  (Hfull : message_dependencies_full_node_condition_prop)
+  s
+  (Hs : valid_state_prop (pre_loaded_with_all_messages_vlsm X) s)
+  : forall dm m, msg_dep_rel dm m ->
+    has_been_observed X s m ->
+    has_been_observed X s dm.
+Proof.
+  intros dm m Hdm [Hsent|Hreceived].
+  - eapply msg_dep_has_been_sent; eassumption.
+  - eapply full_node_has_been_received; eassumption.
+Qed.
+
+End sec_message_dependencies.
+
+Section sec_composite_message_dependencies.
+
+Context
+  {message : Type}
+  (message_dependencies : message -> set message)
+  `{finite.Finite index}
+  (IM : index -> VLSM message)
+  (Hbs : forall i, HasBeenSentCapability (IM i))
+  (Hbr : forall i, HasBeenReceivedCapability (IM i))
+  (Hbo := fun i => HasBeenObservedCapability_from_sent_received (IM i))
+  (HMsgDep : forall i, MessageDependencies message_dependencies (IM i))
+  (Free_Hbs := free_composite_HasBeenSentCapability IM (listing_from_finite index) Hbs)
+  (Free_Hbr := free_composite_HasBeenReceivedCapability IM (listing_from_finite index) Hbr)
+  .
+
+Existing Instance Free_Hbs.
+Existing Instance Free_Hbr.
+
+(** If all of the components satisfy the [MessageDependencies] assumptions,
+then their free composition will also do so.
+*)
+Lemma composite_message_dependencies
+  : MessageDependencies message_dependencies (free_composite_vlsm IM).
+Proof.
+  split.
+  - intros m s Hproduce dm Hdm.
+    destruct Hproduce as [(is, iom) [(i, li) Ht]].
+    cut (@has_been_observed _ (IM i) (Hbo i) (s i) dm)
+    ; [intros [Hsent | Hreceived]; [left | right]; exists i; assumption|].
+    eapply message_dependencies_are_necessary; [apply HMsgDep| |eassumption].
+    exists (is i, iom), li.
+    revert Ht.
+    apply
+      (VLSM_projection_input_valid_transition (preloaded_component_projection IM _))
+      with (lY := li).
+    unfold composite_project_label.
+    cbn.
+    case_decide as Heqi; [|contradiction].
+    replace Heqi with (@eq_refl index i) by (apply Eqdep_dec.UIP_dec; assumption).
+    reflexivity.
+  - intros m Hemit.
+    apply can_emit_composite_project in Hemit as [j Hemitj].
+    eapply message_dependencies_are_sufficient in Hemitj; [| apply HMsgDep].
+    revert Hemitj.
+    eapply VLSM_full_projection_can_emit.
+    apply lift_to_composite_generalized_preloaded_vlsm_full_projection.
+    intuition.
+Qed.
+
+Lemma msg_dep_reflects_free_validity
+  (no_initial_messages_in_IM : no_initial_messages_in_IM_prop IM)
+  (X := free_composite_vlsm IM)
+  : forall dm m, msg_dep_rel message_dependencies dm m ->
+    valid_message_prop X m -> valid_message_prop X dm.
+Proof.
+  intros dm m Hdm.
+  rewrite !emitted_messages_are_valid_iff.
+  intros [[i [[im Him] Heqm]] | Hemit]
+  ; [elim (no_initial_messages_in_IM i im); assumption|].
+  right.
+  pose proof (vlsm_is_pre_loaded_with_False X) as XeqXFalse.
+  apply (VLSM_eq_can_emit XeqXFalse) in Hemit.
+  apply (VLSM_eq_can_emit XeqXFalse).
+  cut (valid_message_prop (pre_loaded_vlsm X (fun _ => False)) dm).
+  {
+    clear -no_initial_messages_in_IM.
+    rewrite emitted_messages_are_valid_iff.
+    intros [[[i [[im Him] Heqm]] | Hpreloaded] | Hemit]
+    ; [elim (no_initial_messages_in_IM i im); assumption|contradiction| assumption].
+  }
+  eapply msg_dep_reflects_validity.
+  - apply composite_message_dependencies.
+  - clear -no_initial_messages_in_IM.
+    intros m [i [[im Him] Heqm]].
+    elim (no_initial_messages_in_IM i im).
+    assumption.
+  - intuition.
+  - eassumption.
+  - apply emitted_messages_are_valid_iff.
+    right.
+    assumption.
+Qed.
+
+Lemma msg_dep_reflects_happens_before_free_validity
+  (no_initial_messages_in_IM : no_initial_messages_in_IM_prop IM)
+  (X := free_composite_vlsm IM)
+  : forall dm m, msg_dep_happens_before message_dependencies dm m ->
+    valid_message_prop X m -> valid_message_prop X dm.
+Proof.
+  apply msg_dep_happens_before_reflect.
+  apply msg_dep_reflects_free_validity.
+  assumption.
+Qed.
+
+Lemma msg_dep_happens_before_composite_no_initial_valid_messages_emitted_by_sender
+  {validator : Type}
+  (sender : message -> option validator)
+  (A : validator -> index)
+  (Hchannel : channel_authentication_prop  IM A sender)
+  (no_initial_messages_in_IM : no_initial_messages_in_IM_prop IM)
+  (X := free_composite_vlsm IM)
+  : forall m, valid_message_prop X m ->
+    forall dm, msg_dep_happens_before message_dependencies dm m ->
+    exists v, sender dm = Some v /\
+      can_emit (pre_loaded_with_all_messages_vlsm (IM (A v))) dm.
+Proof.
+  intros m Hm dm Hdm.
+  cut (valid_message_prop X dm).
+  {
+    clear Hdm.
+    revert dm.
+    apply composite_no_initial_valid_messages_emitted_by_sender; assumption.
+  }
+  revert dm m Hdm Hm.
+  apply msg_dep_reflects_happens_before_free_validity.
+  assumption.
+Qed.
+
+End sec_composite_message_dependencies.
+
+Section sec_sub_composite_message_dependencies.
+
+Context
+  {message : Type}
+  (message_dependencies : message -> set message)
+  `{EqDecision index}
+  (IM : index -> VLSM message)
+  (Hbs : forall i, HasBeenSentCapability (IM i))
+  (Hbr : forall i, HasBeenReceivedCapability (IM i))
+  (Hbo := fun i => HasBeenObservedCapability_from_sent_received (IM i))
+  (HMsgDep : forall i, MessageDependencies message_dependencies (IM i))
+  (indices : set index)
+  (SubFree_Hbs := free_composite_HasBeenSentCapability (sub_IM IM indices) (listing_from_finite (sub_index indices)) (sub_has_been_sent_capabilities IM indices Hbs))
+  (SubFree_Hbr := free_composite_HasBeenReceivedCapability (sub_IM IM indices) (listing_from_finite (sub_index indices)) (sub_has_been_received_capabilities IM indices Hbr))
+  .
+
+Existing Instance SubFree_Hbs.
+Existing Instance SubFree_Hbr.
+
+Lemma sub_composite_message_dependencies
+  : MessageDependencies message_dependencies (free_composite_vlsm (sub_IM IM indices)).
+Proof.
+  apply composite_message_dependencies.
+  intro sub_i.
+  destruct_dec_sig sub_i i Hi Heqsub_i.
+  subst.
+  apply HMsgDep.
+Qed.
+
+Lemma msg_dep_reflects_sub_free_validity
+  (no_initial_messages_in_IM : no_initial_messages_in_IM_prop IM)
+  (P : message -> Prop)
+  (Hreflects : forall dm m, msg_dep_rel message_dependencies dm m -> P m -> P dm)
+  (X := free_composite_vlsm (sub_IM IM indices))
+  : forall dm m, msg_dep_rel message_dependencies dm m ->
+    valid_message_prop (pre_loaded_vlsm X P) m ->
+    valid_message_prop (pre_loaded_vlsm X P) dm.
+Proof.
+  eapply msg_dep_reflects_validity; [..|assumption].
+  - apply sub_composite_message_dependencies.
+  - intros m [sub_i [[im Him] Heqm]].
+    destruct_dec_sig sub_i i Hi Heqsub_i.
+    subst.
+    elim (no_initial_messages_in_IM i im).
+    assumption.
+Qed.
+
+End sec_sub_composite_message_dependencies.
+
+Section sec_full_message_dependencies.
+
+Context
+  {message : Type}
+  .
+
+Class FullMessageDependencies
+  (message_dependencies : message -> set message)
+  (full_message_dependencies : message -> set message)
+  :=
+  { full_message_dependencies_happens_before
+      : forall dm m, dm ∈ full_message_dependencies m <-> msg_dep_happens_before message_dependencies dm m
+  ; full_message_dependencies_irreflexive
+      : forall m, m ∉ full_message_dependencies m
+  ; full_message_dependencies_nodups
+      : forall m, NoDup (full_message_dependencies m)
+  }.
+
+End sec_full_message_dependencies.
+
+Section full_message_dependencies_happens_before.
+
+Context
+  {message : Type}
+  (message_dependencies : message -> set message)
+  (full_message_dependencies : message -> set message)
+  (HFullMsgDep : FullMessageDependencies message_dependencies full_message_dependencies)
+  .
+
+Global Instance msg_dep_happens_before_irrefl : Irreflexive (msg_dep_happens_before message_dependencies).
+Proof.
+  intros m Hm.
+  elim (full_message_dependencies_irreflexive m).
+  eapply full_message_dependencies_happens_before.
+  assumption.
+Qed.
+
+Global Instance msg_dep_happens_before_strict : StrictOrder (msg_dep_happens_before message_dependencies) := {}.
+
+Lemma msg_dep_happens_before_wf : well_founded (msg_dep_happens_before message_dependencies).
+Proof.
+  cut (forall n m, length (full_message_dependencies m) < n -> Acc (msg_dep_happens_before message_dependencies) m).
+  {
+    intros Hn m.
+    apply (Hn (S (length (full_message_dependencies m)))).
+    lia.
+  }
+  induction n as [|n IHn]; [lia|].
+  intros m Hm.
+  constructor.
+  intros dm Hdm.
+  apply IHn.
+  unfold lt.
+  transitivity (length (full_message_dependencies m)); [|lia].
+  replace (S _) with (length (dm :: full_message_dependencies dm))
+    by reflexivity.
+  apply NoDup_subseteq_length.
+  - constructor; [apply full_message_dependencies_irreflexive| apply full_message_dependencies_nodups].
+  - intros m' Hm'.
+    inversion Hm'; subst; [apply full_message_dependencies_happens_before; assumption|].
+    revert H1.
+    setoid_rewrite full_message_dependencies_happens_before.
+    intro Hm'dm.
+    transitivity dm; assumption.
+Qed.
+
+Lemma FullMessageDependencies_ind
+  (P : message -> Prop)
+  m
+  (IHm : forall dm, dm ∈ full_message_dependencies m -> (forall dm0, dm0 ∈ full_message_dependencies dm -> P dm0) -> P dm)
+  : forall dm, dm ∈ full_message_dependencies m -> P dm.
+Proof.
+  induction m using (well_founded_ind msg_dep_happens_before_wf).
+  intros dm Hdm.
+  apply IHm; [assumption|].
+  apply H; [apply full_message_dependencies_happens_before; assumption|].
+  intros dm0 Hdm0.
+  apply IHm.
+  apply full_message_dependencies_happens_before in Hdm.
+  apply full_message_dependencies_happens_before in Hdm0.
+  apply full_message_dependencies_happens_before.
+  change _ with (msg_dep_happens_before message_dependencies dm0 m).
+  transitivity dm; assumption.
+Qed.
+
+End full_message_dependencies_happens_before.
